zoo_parabs/future: Show termination for all futures.

lib/zoo_parabs/future.ml
@@ -1,31 +1,30 @@
 type 'a t =
   ('a, ('a -> unit) Pool.task) Ivar_3.t
 
+let[@inline] set ctx t res =
+  let waiters = Ivar_3.set t res in
+  Lst.iter (fun waiter -> waiter ctx res) waiters
+
 let async ctx task =
   let t = Ivar_3.create () in
-  Pool.async ctx (fun ctx ->
-    let res = task ctx in
-    let waiters = Ivar_3.set t res in
-    Lst.iter (fun waiter -> waiter ctx res) waiters
-  ) ;
+  Pool.async ctx (fun ctx -> set ctx t (task ctx)) ;
   t
 
 let wait ctx t =
   Pool.wait_until ctx (fun () -> Ivar_3.is_set t) ;
   Ivar_3.get t
 
-let iter ctx t fn =
-  match Ivar_3.wait t fn with
+let iter ctx t task =
+  match Ivar_3.wait t task with
   | None ->
       ()
   | Some res ->
-      fn ctx res
+      task ctx res
 
-let map ctx t1 fn =
+let map ctx t1 task =
   let t2 = Ivar_3.create () in
   iter ctx t1 (fun ctx res1 ->
-    let res2 = fn ctx res1 in
-    let waiters = Ivar_3.set t2 res2 in
-    Lst.iter (fun waiter -> waiter ctx res2) waiters
+    Pool.async ctx @@ fun ctx ->
+      set ctx t2 (task ctx res1)
   ) ;
   t2
