theories/zoo_parabs/future.v
@@ -2,6 +2,8 @@ From zoo Require Import
   prelude.
 From zoo.iris.bi Require Import
   big_op.
+From zoo.iris.base_logic Require Import
+  lib.saved_prop.
 From zoo.language Require Import
   notations.
 From zoo.diaframe Require Import
@@ -18,16 +20,20 @@ From zoo Require Import
   options.
 
 Implicit Types b : bool.
-Implicit Types v t pool ctx task waiter fn : val.
+Implicit Types depth : nat.
+Implicit Types v t pool ctx task waiter : val.
 Implicit Types scope : pool_scope.
-Implicit Types ω : unit.
+Implicit Types ω : gname.
+Implicit Types ωs : list gname.
 
 Class FutureG Σ `{pool_G : PoolG Σ} := {
-  #[local] future_G_ivar_G :: Ivar3G Σ unit ;
+  #[local] future_G_ivar_G :: Ivar3G Σ gname ;
+  #[local] future_G_saved_prop_G :: SavedPropG Σ ;
 }.
 
 Definition future_Σ := #[
-  ivar_3_Σ unit
+  ivar_3_Σ gname ;
+  saved_prop_Σ
 ].
 #[global] Instance subG_future_Σ Σ `{pool_G : PoolG Σ} :
   subG future_Σ Σ →
@@ -39,6 +45,7 @@ Qed.
 Section future_G.
   Context `{future_G : FutureG Σ}.
 
+  Implicit Types P : iProp Σ.
   Implicit Types Ψ Χ Ξ : val → iProp Σ.
 
   #[local] Definition waiter_model pool t waiter ω : iProp Σ :=
@@ -46,29 +53,95 @@ Section future_G.
     pool_context pool ctx scope -∗
     ivar_3_result t v -∗
     WP waiter ctx v {{ res,
+      ∃ P,
       ⌜res = ()%V⌝ ∗
-      pool_context pool ctx scope
+      pool_context pool ctx scope ∗
+      saved_prop ω P ∗
+      ▷ □ P
     }}.
-  Definition future_inv pool t Ψ Ξ :=
-    ivar_3_inv t Ψ Ξ (waiter_model pool).
+
+  #[local] Definition receipt_1 t : iProp Σ :=
+    ∃ waiters ωs,
+    ivar_3_resolved t ∗
+    ivar_3_waiters t waiters ωs ∗
+    [∗ list] ω ∈ ωs,
+      ∃ P,
+      saved_prop ω P ∗
+      □ P.
+  #[local] Instance : CustomIpatFormat "receipt_1" :=
+    " ( %waiters &
+        %ωs &
+        #H{{}_}resolved &
+        #H{{}_}waiters &
+        #Hωs
+      )
+    ".
+  #[local] Definition receipt_2 pool t :=
+    pool_obligation pool (receipt_1 t).
+
+  #[local] Fixpoint future_inv pool t depth Ψ Ξ : iProp Σ :=
+    ivar_3_inv t Ψ Ξ (waiter_model pool) ∗
+    match depth with
+    | 0 =>
+        receipt_2 pool t
+    | S depth =>
+          □ receipt_2 pool t
+        ∨ ∃ parent Ψ_parent Ξ_parent waiter ω,
+          future_inv pool parent depth Ψ_parent Ξ_parent ∗
+          ivar_3_waiter parent waiter ω ∗
+          saved_prop ω (receipt_2 pool t)
+    end.
+  #[local] Instance : CustomIpatFormat "inv" :=
+    " ( #H{{}_}inv &
+        H{{}_}receipt
+      )
+    ".
+
+  Definition future_obligation pool depth P : iProp Σ :=
+      □ P
+    ∨ ∃ t Ψ Ξ waiter ω,
+      future_inv pool t depth Ψ Ξ ∗
+      ivar_3_waiter t waiter ω ∗
+      saved_prop ω P.
+  #[local] Instance : CustomIpatFormat "obligation" :=
+    " [ #HP
+      | ( %{;t} &
+          %Ψ{_{}} &
+          %Ξ{_{}} &
+          %waiter &
+          %ω &
+          #H{{}_}inv &
+          #H{{}_}waiter &
+          #Hω
+        )
+      ]
+    ".
+
+  #[local] Definition receipt_3 pool t depth :=
+    match depth with
+    | 0 =>
+        receipt_2 pool t
+    | S depth =>
+        future_obligation pool depth (receipt_2 pool t)
+    end.
 
   Definition future_consumer :=
     ivar_3_consumer.
 
   Definition future_result :=
     ivar_3_result.
-  Definition future_finished t : iProp Σ :=
+  Definition future_resolved t : iProp Σ :=
     ∃ v,
     future_result t v.
 
-  #[global] Instance future_proper pool t :
+  #[local] Instance future_inv_proper pool t depth :
     Proper (
       (pointwise_relation _ (≡)) ==>
       (pointwise_relation _ (≡)) ==>
       (≡)
-    ) (future_inv pool t).
+    ) (future_inv pool t depth).
   Proof.
-    solve_proper.
+    destruct depth; solve_proper.
   Qed.
 
   #[global] Instance future_result_timeless t v :
@@ -77,8 +150,13 @@ Section future_G.
     apply _.
   Qed.
 
-  #[global] Instance future_inv_persistent pool t Ψ Ξ :
-    Persistent (future_inv pool t Ψ Ξ).
+  #[global] Instance future_inv_persistent pool t depth Ψ Ξ :
+    Persistent (future_inv pool t depth Ψ Ξ).
+  Proof.
+    move: t Ψ Ξ. induction depth; apply _.
+  Qed.
+  #[global] Instance future_obligation_persistent pool depth P :
+    Persistent (future_obligation pool depth P).
   Proof.
     apply _.
   Qed.
@@ -88,22 +166,99 @@ Section future_G.
     apply _.
   Qed.
 
-  Lemma future_consumer_divide {pool t Ψ Ξ Χ} Χs :
-    future_inv pool t Ψ Ξ -∗
+  #[local] Lemma future_inv_unfold pool t depth Ψ Ξ :
+    future_inv pool t depth Ψ Ξ ⊣⊢
+      ivar_3_inv t Ψ Ξ (waiter_model pool) ∗
+      receipt_3 pool t depth.
+  Proof.
+    destruct depth as [| depth].
+    all: iSplit.
+    all: iIntros "(:inv)".
+    all: iFrame "#∗".
+  Qed.
+
+  #[local] Lemma future_inv_finished_receipt pool t depth Ψ Ξ :
+    future_inv pool t depth Ψ Ξ -∗
+    pool_finished pool -∗
+    ▷^(2 * depth + 1) receipt_1 t.
+  Proof.
+    iInduction depth as [| depth] "IH" forall (t Ψ Ξ).
+    all: rewrite future_inv_unfold.
+    all: iIntros "(:inv =t) #Hpool_finished".
+
+    - iDestruct (pool_obligation_finished with "Ht_receipt Hpool_finished") as "Ht_receipt".
+      iNext => //.
+
+    - iDestruct "Ht_receipt" as "(:obligation =parent)".
+
+      + iDestruct (pool_obligation_finished with "HP Hpool_finished") as "Hreceipt".
+        iNext => //.
+
+      + iDestruct ("IH" with "Hparent_inv Hpool_finished") as "(:receipt_1 =parent)".
+
+        iEval (replace (2 * S depth + 1) with (2 * depth + 1 + 2) by lia).
+        iEval (rewrite bi.laterN_add).
+        iNext.
+
+        iDestruct (ivar_3_waiter_valid with "Hparent_waiters Hparent_waiter") as %(i & _ & Hωs_lookup).
+        iDestruct (big_sepL_lookup with "Hωs") as "(%P & Hω_ & -#Hreceipt)"; first done.
+        iDestruct (saved_prop_agree with "Hω Hω_") as "Heq".
+        iNext.
+        iRewrite -"Heq" in "Hreceipt".
+
+        iDestruct (pool_obligation_finished with "Hreceipt Hpool_finished") as "Hreceipt".
+        iNext => //.
+  Qed.
+  Lemma future_inv_finished pool t depth Ψ Ξ :
+    future_inv pool t depth Ψ Ξ -∗
+    pool_finished pool -∗
+    ▷^(2 * depth + 1) future_resolved t.
+  Proof.
+    iIntros "Hinv Hpool_finished".
+    iDestruct (future_inv_finished_receipt with "Hinv Hpool_finished") as "(:receipt_1)".
+    auto.
+  Qed.
+
+  Lemma future_obligation_finished pool depth P :
+    future_obligation pool depth P -∗
+    pool_finished pool -∗
+    ▷^(2 * depth + 2) □ P.
+  Proof.
+    iIntros "(:obligation) Hpool_finished //".
+
+    iDestruct (future_inv_finished_receipt with "Hinv Hpool_finished") as "(:receipt_1)".
+
+    iEval (replace (2 * depth + 2) with (2 * depth + 1 + 1) by lia).
+    iEval (rewrite bi.laterN_add).
+    iNext.
+
+    iDestruct (ivar_3_waiter_valid with "Hwaiters Hwaiter") as %(i & _ & Hωs_lookup).
+    iDestruct (big_sepL_lookup with "Hωs") as "(%P_ & Hω_ & HP)"; first done.
+    iDestruct (saved_prop_agree with "Hω Hω_") as "Heq".
+    iNext.
+    iRewrite -"Heq" in "HP" => //.
+  Qed.
+
+  Lemma future_consumer_divide {pool t depth Ψ Ξ Χ} Χs :
+    future_inv pool t depth Ψ Ξ -∗
     future_consumer t Χ -∗
     (∀ x, Χ x -∗ [∗ list] Χ ∈ Χs, Χ x) ={⊤}=∗
     [∗ list] Χ ∈ Χs, future_consumer t Χ.
   Proof.
-    apply ivar_3_consumer_divide.
+    rewrite future_inv_unfold.
+    iIntros "(:inv)".
+    iApply (ivar_3_consumer_divide with "Hinv").
   Qed.
-  Lemma future_consumer_split {pool t Ψ Χ Ξ} Χ1 Χ2 :
-    future_inv pool t Ψ Ξ -∗
+  Lemma future_consumer_split {pool t depth Ψ Χ Ξ} Χ1 Χ2 :
+    future_inv pool t depth Ψ Ξ -∗
     future_consumer t Χ -∗
     (∀ v, Χ v -∗ Χ1 v ∗ Χ2 v) ={⊤}=∗
       future_consumer t Χ1 ∗
       future_consumer t Χ2.
   Proof.
-    apply ivar_3_consumer_split.
+    rewrite future_inv_unfold.
+    iIntros "(:inv)".
+    iApply (ivar_3_consumer_split with "Hinv").
   Qed.
 
   Lemma future_result_agree t v1 v2 :
@@ -114,16 +269,18 @@ Section future_G.
     apply ivar_3_result_agree.
   Qed.
 
-  Lemma future_inv_result pool t Ψ Ξ v :
-    future_inv pool t Ψ Ξ -∗
+  Lemma future_inv_result pool t depth Ψ Ξ v :
+    future_inv pool t depth Ψ Ξ -∗
     future_result t v ={⊤}=∗
     ▷ □ Ξ v.
   Proof.
-    apply ivar_3_inv_result.
+    rewrite future_inv_unfold.
+    iIntros "(:inv) Hresult".
+    iApply (ivar_3_inv_result with "Hinv Hresult").
   Qed.
-  Lemma future_inv_result' pool t Ψ Ξ v :
+  Lemma future_inv_result' pool t depth Ψ Ξ v :
     £ 1 -∗
-    future_inv pool t Ψ Ξ -∗
+    future_inv pool t depth Ψ Ξ -∗
     future_result t v ={⊤}=∗
     □ Ξ v.
   Proof.
@@ -131,18 +288,20 @@ Section future_G.
     iMod (future_inv_result with "Hfut_inv Hfut_result") as "HΞ".
     iApply (lc_fupd_elim_later with "H£ HΞ").
   Qed.
-  Lemma future_inv_result_consumer pool t Ψ Ξ v Χ :
-    future_inv pool t Ψ Ξ -∗
+  Lemma future_inv_result_consumer pool t depth Ψ Ξ v Χ :
+    future_inv pool t depth Ψ Ξ -∗
     future_result t v -∗
     future_consumer t Χ ={⊤}=∗
       ▷^2 Χ v ∗
       ▷ □ Ξ v.
   Proof.
-    apply ivar_3_inv_result_consumer.
+    rewrite future_inv_unfold.
+    iIntros "(:inv) Hresult Hconsumer".
+    iApply (ivar_3_inv_result_consumer with "Hinv Hresult Hconsumer").
   Qed.
-  Lemma future_inv_result_consumer' pool t Ψ Ξ v Χ :
+  Lemma future_inv_result_consumer' pool t depth Ψ Ξ v Χ :
     £ 2 -∗
-    future_inv pool t Ψ Ξ -∗
+    future_inv pool t depth Ψ Ξ -∗
     future_result t v -∗
     future_consumer t Χ ={⊤}=∗
       Χ v ∗
@@ -153,6 +312,59 @@ Section future_G.
     rewrite -bi.later_sep.
     iMod (lc_fupd_elim_later with "H£1 H") as "(HΧ & $)".
     iApply (lc_fupd_elim_later with "H£2 HΧ").
+  Qed.
+
+  #[local] Lemma future_set_spec pool ctx scope t Ψ Ξ v :
+    {{{
+      pool_context pool ctx scope ∗
+      ivar_3_inv t Ψ Ξ (waiter_model pool) ∗
+      ivar_3_producer t ∗
+      ▷ Ψ v ∗
+      ▷ □ Ξ v
+    }}}
+      future_set ctx t v
+    {{{
+      RET ();
+      pool_context pool ctx scope ∗
+      receipt_1 t
+    }}}.
+  Proof.
+    iIntros "%Φ (Hctx & #Hinv & Hproducer & HΨ & HΞ) HΦ".
+
+    wp_rec.
+    wp_smart_apply (ivar_3_set_spec with "[$Hinv $Hproducer $HΨ $HΞ]") as (waiters ωs) "(#Hresult & #Hwaiters & Hwaiter_models)".
+
+    iDestruct (big_sepL2_length with "Hwaiter_models") as %Hlength.
+
+    wp_smart_apply (lst_iter_spec (λ i _,
+      pool_context pool ctx scope ∗
+      ( [∗ list] ω ∈ take i ωs,
+        ∃ P,
+        saved_prop ω P ∗
+        □ P
+      ) ∗
+      ( [∗ list] waiter; ω ∈ drop i waiters; drop i ωs,
+        waiter_model pool t waiter ω
+      )
+    )%I with "[$Hctx Hwaiter_models]") as "(Hctx & #Hωs & _)"; first done.
+    { iStep.
+      iIntros "!> %i %waiter %Hwaiters_lookup (Hctx & Hωs & Hwaiter_models)".
+
+      iEval (rewrite (drop_S waiters waiter) //) in "Hwaiter_models".
+      iDestruct (big_sepL2_cons_inv_l with "Hwaiter_models") as "(%ω & %ωs' & %Heq & Hwaiter_model & Hwaiter_models)".
+      apply drop_cons_inv in Heq as (Hωs_lookup & ->).
+
+      wp_smart_apply (wp_wand with "(Hwaiter_model Hctx Hresult)") as (res) "(%P & -> & $ & Hω & HP)".
+
+      iFrameStep.
+      iEval (rewrite (take_S_r _ _ ω) //).
+      iApply big_sepL_snoc.
+      iFrame.
+    }
+    iEval (rewrite Hlength firstn_all) in "Hωs".
+
+    iApply "HΦ".
+    iFrame "#∗".
   Qed.
 
   Lemma future_async_spec Ψ Ξ pool ctx scope task :
@@ -171,40 +383,30 @@ Section future_G.
     {{{ t,
       RET t;
       pool_context pool ctx scope ∗
-      future_inv pool t Ψ Ξ ∗
-      future_consumer t Ψ ∗
-      pool_obligation pool (future_finished t)
+      future_inv pool t 0 Ψ Ξ ∗
+      future_consumer t Ψ
     }}}.
   Proof.
     iIntros "%Φ (Hctx & Htask) HΦ".
 
     wp_rec.
-    wp_smart_apply (ivar_3_create_spec Ψ Ξ with "[//]") as (ivar) "(#Hivar_inv & Hivar_producer & Hivar_consumer)".
+    wp_smart_apply (ivar_3_create_spec Ψ Ξ (waiter_model pool) with "[//]") as (t) "(#Hinv & Hproducer & Hconsumer)".
 
     wp_smart_apply (pool_async_spec (
-      ivar_3_resolved ivar
-    ) with "[$Hctx Htask Hivar_producer]") as "(Hctx & Hobligation)".
-    { clear ctx scope. iIntros "%ctx %scope Hctx".
-
+      receipt_1 t
+    ) with "[$Hctx Htask Hproducer]") as "(Hctx & Hreceipt)".
+    { iIntros "{%} %ctx %scope Hctx".
       wp_smart_apply (wp_wand with "(Htask Hctx)") as (v) "(Hctx & HΨ & HΞ)".
-      wp_smart_apply (ivar_3_set_spec with "[$Hivar_inv $Hivar_producer $HΨ $HΞ]") as (waiters ωs) "(#Hivar_result & _ & Hwaiters)".
-
-      wp_smart_apply (lst_iter_spec' (λ _ _, pool_context pool ctx scope)%I with "[$Hctx Hwaiters]") as "$"; first done.
-      { iDestruct (big_sepL2_retract_r with "Hwaiters") as "(_ & Hwaiters)".
-        iApply (big_sepL_impl with "Hwaiters").
-        iSteps.
-      }
-
-      iFrame "#∗".
+      wp_apply (future_set_spec with "[$]") as "($ & #$)".
     }
 
     iSteps.
   Qed.
 
-  Lemma future_wait_spec pool ctx scope t Ψ Ξ :
+  Lemma future_wait_spec pool ctx scope t depth Ψ Ξ :
     {{{
       pool_context pool ctx scope ∗
-      future_inv pool t Ψ Ξ
+      future_inv pool t depth Ψ Ξ
     }}}
       future_wait ctx t
     {{{ v,
@@ -214,88 +416,119 @@ Section future_G.
       future_result t v
     }}}.
   Proof.
-    iIntros "%Φ (Hctx & #Hivar_inv) HΦ".
+    setoid_rewrite future_inv_unfold.
+    iIntros "%Φ (Hctx & (:inv)) HΦ".
 
     wp_rec.
 
-    wp_smart_apply (pool_wait_until_spec (ivar_3_resolved t)%I with "[$Hctx]") as "(Hctx & %v & #Hivar_result)".
+    wp_smart_apply (pool_wait_until_spec (
+      ivar_3_resolved t
+    )%I with "[$Hctx]") as "(Hctx & %v & #Hresult)".
     { iModIntro.
-      wp_smart_apply (ivar_3_is_set_spec with "Hivar_inv") as (b) "Hivar_result".
+      wp_smart_apply (ivar_3_is_set_spec with "Hinv") as (b) "Hresult".
       rewrite /ivar_3_resolved. destruct b; iSteps.
     }
 
-    wp_smart_apply (ivar_3_get_spec with "[$Hivar_inv $Hivar_result]") as "H£".
+    wp_smart_apply (ivar_3_get_spec with "[$Hinv $Hresult]") as "H£".
     iSteps.
   Qed.
 
-  Lemma future_iter_spec pool ctx scope t Ψ Ξ fn :
+  Lemma future_iter_spec P pool ctx scope t depth Ψ Ξ task :
     {{{
       pool_context pool ctx scope ∗
-      future_inv pool t Ψ Ξ ∗
+      future_inv pool t depth Ψ Ξ ∗
       ( ∀ ctx scope v,
         pool_context pool ctx scope -∗
         future_result t v -∗
-        WP fn ctx v {{ res,
+        WP task ctx v {{ res,
           ⌜res = ()%V⌝ ∗
-          pool_context pool ctx scope
+          pool_context pool ctx scope ∗
+          ▷ □ P
         }}
       )
     }}}
-      future_iter ctx t fn
+      future_iter ctx t task
     {{{
       RET ();
-      pool_context pool ctx scope
+      pool_context pool ctx scope ∗
+      future_obligation pool depth P
     }}}.
   Proof.
-    iIntros "%Φ (Hctx & #Hivar_inv & Hfn) HΦ".
+    setoid_rewrite future_inv_unfold.
+    iIntros "%Φ (Hctx & (:inv) & Htask) HΦ".
 
-    wp_rec.
-    wp_smart_apply (ivar_3_wait_spec inhabitant with "[$Hivar_inv $Hfn]") as ([v |]) "H"; iSteps.
+    wp_rec credit:"H£".
+
+    iMod (saved_prop_alloc P) as "(%ω & #Hω)".
+    wp_smart_apply (ivar_3_wait_spec ω with "[$Hinv Htask]") as ([v |]) "H".
+    { iIntros "{%} !> %ctx %scope %v Hctx #Hresult".
+      wp_apply (wp_wand with "(Htask Hctx Hresult)").
+      iSteps.
+    }
+
+    - iDestruct "H" as "(_ & #Hresult & Hwaiter_model)".
+
+      iApply wp_fupd.
+      wp_smart_apply (wp_wand with "(Hwaiter_model Hctx Hresult)") as (res) "(%P_ & -> & Hctx & Hω_ & HP)".
+
+      iApply "HΦ".
+      iDestruct (saved_prop_agree with "Hω Hω_") as "Heq".
+      iMod (lc_fupd_elim_later with "H£ [HP Heq]") as "H".
+      { iNext. iAccu. }
+      iDestruct "H" as "(#HP & Heq)".
+      iRewrite -"Heq" in "HP".
+      iFrameSteps.
+
+    - wp_pures.
+
+      iApply "HΦ".
+      iFrame. iRight. iExists t, Ψ, Ξ, task, ω.
+      rewrite future_inv_unfold. iFrameSteps.
   Qed.
 
-  Lemma future_map_spec {pool ctx scope t1 Ψ1 Ξ1} Ψ2 Ξ2 fn :
+  Lemma future_map_spec {pool ctx scope t1 depth Ψ1 Ξ1} Ψ2 Ξ2 task :
     {{{
       pool_context pool ctx scope ∗
-      future_inv pool t1 Ψ1 Ξ1 ∗
+      future_inv pool t1 depth Ψ1 Ξ1 ∗
       ( ∀ ctx scope v1,
         pool_context pool ctx scope -∗
         future_result t1 v1 -∗
-        WP fn ctx v1 {{ v2,
+        WP task ctx v1 {{ v2,
           pool_context pool ctx scope ∗
           ▷ Ψ2 v2 ∗
           ▷ □ Ξ2 v2
         }}
       )
     }}}
-      future_map ctx t1 fn
+      future_map ctx t1 task
     {{{ t2,
       RET t2;
       pool_context pool ctx scope ∗
-      future_inv pool t2 Ψ2 Ξ2 ∗
+      future_inv pool t2 (S depth) Ψ2 Ξ2 ∗
       future_consumer t2 Ψ2
     }}}.
   Proof.
-    iIntros "%Φ (Hctx & #Ht1_inv & Hfn) HΦ".
+    iIntros "%Φ (Hctx & #Ht1_inv & Htask) HΦ".
 
     wp_rec.
-    wp_smart_apply (ivar_3_create_spec Ψ2 Ξ2 with "[//]") as (t2) "(#Hivar2_inv & Hivar2_producer & Hivar2_consumer)".
+    wp_smart_apply (ivar_3_create_spec Ψ2 Ξ2 (waiter_model pool) with "[//]") as (t2) "(#Ht2_inv & Ht2_producer & Ht2_consumer)".
 
-    wp_smart_apply (future_iter_spec with "[$Hctx $Ht1_inv Hfn Hivar2_producer]") as "Hctx".
-    { clear ctx scope. iIntros "%ctx %scope %v1 Hctx #Ht1_result".
-
-      wp_smart_apply (wp_wand with "(Hfn Hctx Ht1_result)") as (v2) "(Hctx & HΨ2 & HΞ2)".
-      wp_smart_apply (ivar_3_set_spec with "[$Hivar2_inv $Hivar2_producer $HΨ2 $HΞ2]") as (waiters ωs) "(#Hivar2_result & _ & Hwaiters)".
-
-      wp_smart_apply (lst_iter_spec' (λ _ _, pool_context pool ctx scope)%I with "[$Hctx Hwaiters]") as "$"; first done.
-      { iDestruct (big_sepL2_retract_r with "Hwaiters") as "(_ & Hwaiters)".
-        iApply (big_sepL_impl with "Hwaiters").
-        iSteps.
+    wp_smart_apply (future_iter_spec (
+      receipt_2 pool t2
+    ) with "[$Hctx $Ht1_inv Htask Ht2_producer]") as "(Hctx & Hobligation)".
+    { iIntros "{%} %ctx %scope %v1 Hctx #Ht1_result".
+      wp_smart_apply (pool_async_spec (
+        receipt_1 t2
+      ) with "[$Hctx Htask Ht2_producer]") as "($ & #$) //".
+      { iIntros "{%} %ctx %scope Hctx".
+        wp_smart_apply (wp_wand with "(Htask Hctx Ht1_result)") as (v2) "(Hctx & HΨ2 & HΞ2)".
+        wp_apply (future_set_spec with "[$]") as "($ & #$)".
       }
-
-      iSteps.
     }
 
-    iSteps.
+    wp_pures.
+
+    iStepFrameSteps.
   Qed.
 End future_G.
 
@@ -303,5 +536,6 @@ From zoo_parabs Require
   future__opaque.
 
 #[global] Opaque future_inv.
+#[global] Opaque future_obligation.
 #[global] Opaque future_consumer.
 #[global] Opaque future_result.
